\documentclass{article}

\title{Jane Street Puzzle}
\author{Brandon Chinn}
\date{February 2024}

% Macros
\newcommand{\dz}{{\; \mathrm{d}z}}
\newcommand{\dx}{{\; \mathrm{d}x}}
\newcommand{\otherwise}{{\mathrm{otherwise}}}

% Formatting
\usepackage{amsmath}
\usepackage{parskip}

\begin{document}
\maketitle

\section{Problem}

Given two random points in a square, what is the probability that the circle formed by the two points goes outside the square?

\section{Notation}

Probability density functions will be notated as $f_X(z)$, and cumulative density functions will be notated as $F_X(t)$. $F_X(t)$ is equivalent to $P[X \leq t]$.

PDFs are defined to be 0 if the variable is outside the range of all of the cases. CDFs are defined to be 0 if the variable is less than the range of all the cases, and 1 if the variable is greater than the range of all the cases.

\section{Definitions}

\begin{gather*}
    x_1, x_2, y_1, y_2 = [0, 1] \\
    O_x = \frac{x_1 + x_2}{2} \\
    O_y = \frac{y_1 + y_2}{2} \\
    d = \sqrt{(x_2 - x_1)^2 + (y_2 - y_1)^2} \\
    r = \frac{d}{2} \\
\end{gather*}

The solution is the value of the following probability:

\begin{align*}
  1 - P[(0 \leq O_x \pm r \leq 1) \land (0 \leq O_y \pm r \leq 1)] \\
= 1 - P[(0 \leq O_x - r) \land (O_x + r \leq 1) \land (0 \leq O_y - r) \land (O_y + r \leq 1)] \\
\end{align*}

\section{Probability of points}

\begin{align*}
f_{x_1}(z) = f_{x_2}(z) = f_{y_1}(z) = f_{y_2}(z) &=
\begin{cases}
    1 & 0 \leq z \leq 1
\end{cases}
\\
F_{x_1}(t) = F_{x_2}(t) = F_{y_1}(t) = F_{y_2}(t) &=
\begin{cases}
    t & 0 \leq t \leq 1
\end{cases}
\end{align*}

\section{Probability of $x_1 + x_2$ and $y_1 + y_2$}

From the definition of convolution on two uniform distributions:

\begin{align*}
f_{x_1 + x_2}(z) &= f_{y_1 + y_2}(z) =
\begin{cases}
    z     & 0 \leq z \leq 1 \\
    2 - z & 1 \leq z \leq 2 \\
\end{cases}
\end{align*}

When $z \in [0, 1]$:

\begin{align*}
F_{x_1 + x_2}(t)
&= \int_{0}^{t} z \dz \\
&= \frac{1}{2}z^2 \Big|_{0}^{t} \\
&= \frac{1}{2}t^2 - \frac{1}{2}0^2 \\
&= \frac{1}{2}t^2 \\
\end{align*}

When $z \in [1, 2]$:

\begin{align*}
F_{x_1 + x_2}(t)
&= \int_{0}^{1} z \dz + \int_{1}^{t} 2 - z \dz \\
&= \left[ \frac{1}{2}z^2 \right]_{0}^{1} + \left[ 2z - \frac{1}{2}z^2 \right]_{1}^{t} \\
&= \left[ \frac{1}{2}1^2 - \frac{1}{2}0^2 \right] + \left[ \left( 2t - \frac{1}{2}t^2 \right) - \left( 2(1) - \frac{1}{2}1^2 \right) \right] \\
&= \frac{1}{2} + 2t - \frac{1}{2}t^2 - \frac{3}{2} \\
&= -\frac{1}{2}t^2 + 2t - 1 \\
\end{align*}

Putting it together:

\begin{align*}
F_{x_1 + x_2}(t) &= F_{y_1 + y_2}(t) =
\begin{cases}
    \frac{1}{2}t^2           & 0 \leq t \leq 1 \\
    -\frac{1}{2}t^2 + 2t - 1 & 1 \leq t \leq 2 \\
\end{cases}
\end{align*}

\section{Probability of $O_x$ and $O_y$}

To find the CDF of the origin:

\begin{align*}
F_{O_x}(t)
&= P \left[ O_x \leq t \right] \\
&= P \left[ \frac{x_1 + x_2}{2} \leq t \right] \\
&= P \left[ x_1 + x_2 \leq 2t \right] \\
&= F_{x_1 + x_2}(2t) \\
\end{align*}

When $t \in [0, 1]$:

\begin{align*}
F_{x_1 + x_2}(2t)
&= \frac{1}{2}(2t)^2 \\
&= 2t^2 \\
\end{align*}

When $t \in [1, 2]$:

\begin{align*}
F_{x_1 + x_2}(2t)
&= -\frac{1}{2}(2t)^2 + 2(2t) - 1 \\
&= -2t^2 + 4t - 1 \\
\end{align*}

Putting it together:

\begin{align*}
F_{O_x}(t) &= F_{O_y}(t) =
\begin{cases}
    2t^2           & 0 \leq t \leq \frac{1}{2} \\
    -2t^2 + 4t - 1 & \frac{1}{2} \leq t \leq 1 \\
\end{cases}
\\
f_{O_x}(z) &= f_{O_y}(z) =
\begin{cases}
    4z      & 0 \leq z \leq \frac{1}{2} \\
    -4z + 4 & \frac{1}{2} \leq z \leq 1 \\
\end{cases}
\end{align*}

\section{Probability of $-x_1$ and $-y_1$}

\begin{align*}
F_{-x_1}(t)
&= P \left[ -x_1 \leq t \right] \\
&= P \left[ x_1 > -t \right] \\
&= 1 - P \left[ x_1 \leq -t \right] \\
&= 1 - F_{x_1}(-t) \\
&= 1 - (-t) \\
&= t + 1 \\
\end{align*}

Therefore:

\begin{align*}
F_{-x_1}(t) &= F_{-y_1}(t) =
\begin{cases}
    t + 1 & -1 \leq t \leq 0 \\
\end{cases}
\\
f_{-x_1}(z) &= f_{-y_1}(z) =
\begin{cases}
    1 & -1 \leq z \leq 0 \\
\end{cases}
\end{align*}

\section{Probability of $x_2 - x_1$ and $y_2 - y_1$}

New range is $[-1, 1]$.

\begin{align*}
f_{x_2 - x_1}(z)
&= \int_{-\inf}^{\inf} f_{x_2}(x)f_{-x_1}(z - x) \dx \\
&= \int_{0}^{1} f_{x_2}(x)f_{-x_1}(z - x) \dx \\
\end{align*}

When $z \in [-1, 0]$:

\begin{align*}
&= \int_{0}^{z + 1} f_{x_2}(x)f_{-x_1}(z - x) \dx \\
&= \int_{0}^{z + 1} (1)(1) \dx \\
&= x \Big|_{0}^{z + 1} \\
&= z + 1 \\
\end{align*}

When $z \in [0, 1]$:

\begin{align*}
&= \int_{z}^{1} f_{x_2}(x)f_{-x_1}(z - x) \dx \\
&= \int_{z}^{1} (1)(1) \dx \\
&= x \Big|_{z}^{1} \\
&= 1 - z \\
\end{align*}

Putting it together:

\begin{align*}
f_{x_2 - x_1}(z) &= f_{y_2 - y_1}(z) =
\begin{cases}
    z + 1 & -1 \leq z \leq 0 \\
    1 - z & 0 \leq z \leq 1 \\
\end{cases}
\\
F_{x_2 - x_1}(t) &= F_{y_2 - y_1}(t) =
\begin{cases}
    \frac{1}{2}t^2 + t + \frac{1}{2}  & -1 \leq t \leq 0 \\
    -\frac{1}{2}t^2 + t + \frac{1}{2} & 0 \leq t \leq 1 \\
\end{cases}
\end{align*}

\section{Probability of $(x_2 - x_1)^2$ and $(y_2 - y_1)^2$}

\begin{align*}
F_{(x_2 - x_1)^2}(t)
&= P \left[ (x_2 - x_1)^2 \leq t \right] \\
&= P \left[ x_2 - x_1 \leq \pm \sqrt{t} \right] \\
&= P \left[ \left( -\sqrt{t} \leq x_2 - x_1 \leq 0 \right) \land \left( 0 \leq x_2 - x_1 \leq \sqrt{t} \right) \right] \\
\end{align*}

When $x_2 - x_1 \in [-1, 0]$:

\begin{align*}
&= P \left[ -\sqrt{t} \leq x_2 - x_1 \leq 0 \right] \\
&= F_{x_2 - x_1}(0) - F_{x_2 - x_1}(-\sqrt{t}) \\
&= \left( -\frac{1}{2}0^2 + 0 + \frac{1}{2} \right) - \left( -\frac{1}{2}(-\sqrt{t})^2 + (-\sqrt{t}) + \frac{1}{2} \right) \\
&= \frac{1}{2} + \frac{1}{2}t + \sqrt{t} - \frac{1}{2} \\
&= \frac{1}{2}t + \sqrt{t} \\
\end{align*}

When $x_2 - x_1 \in [0, 1]$:

\begin{align*}
&= P \left[ 0 \leq x_2 - x_1 \leq \sqrt{t} \right] \\
&= F_{x_2 - x_1}(\sqrt{t}) - F_{x_2 - x_1}(0) \\
&= \left( -\frac{1}{2}(\sqrt{t})^2 + \sqrt{t} + \frac{1}{2} \right) - \left( -\frac{1}{2}(0)^2 + 0 + \frac{1}{2} \right) \\
&= -\frac{1}{2}t + \sqrt{t} \\
\end{align*}

Putting it together:

\begin{align*}
F_{(x_2 - x_1)^2}(t) = F_{(y_2 - y_1)^2}(t)
&=
\begin{cases}
    \left( -\frac{1}{2}t + \sqrt{t} \right)
    + \left( -\frac{1}{2}t + \sqrt{t} \right)
    & 0 \leq t \leq 1 \\
\end{cases}
\\
&=
\begin{cases}
    -t + 2\sqrt{t} & 0 \leq t \leq 1 \\
\end{cases}
\\
f_{(x_2 - x_1)^2}(z) &= f_{(y_2 - y_1)^2}(z) =
\begin{cases}
    -1 + z^{-\frac{1}{2}} & 0 \leq z \leq 1 \\
\end{cases}
\end{align*}

\section{Probability of $(x_2 - x_1)^2 + (y_2 - y_1)^2$}

\begin{align*}
f_{(x_2 - x_1)^2 + (y_2 - y_1)^2}(z)
&= \int_{-\inf}^{\inf} f_{(x_2 - x_1)^2}(x)f_{(y_2 - y_1)^2}(z - x) \dx \\
&= \int_{0}^{1} f_{(x_2 - x_1)^2}(x)f_{(y_2 - y_1)^2}(z - x) \dx \\
\end{align*}

When $z \in [0, 1]$:

\begin{align*}
&= \int_{0}^{z} f_{(x_2 - x_1)^2}(x)f_{(y_2 - y_1)^2}(z - x) \dx \\
&= \int_{0}^{z} \left( \frac{1}{\sqrt{x}} - 1 \right) \left( \frac{1}{\sqrt{z - x}} - 1 \right) \dx \\
&= \int_{0}^{z} \frac{1}{\sqrt{xz - x^2}} - \frac{1}{\sqrt{x}} - \frac{1}{\sqrt{z - x}} + 1 \dx \\
&= 2 \sin^{-1} \left( \sqrt{\frac{x}{z}} \right) + 2\sqrt{z - x} - 2\sqrt{x} + x \Big|_{0}^{z} \\
&= \left( 2 \sin^{-1} \left( \sqrt{\frac{z}{z}} \right) + 2\sqrt{z - z} - 2\sqrt{z} + z \right) - \left( 2 \sin^{-1} \left( \sqrt{\frac{0}{z}} \right) + 2\sqrt{z - 0} - 2\sqrt{0} + 0 \right) \\
&= \pi - 2\sqrt{z} + z - 2\sqrt{z} \\
&= \pi - 4\sqrt{z} + z \\
\end{align*}

When $z \in [1, 2]$:

\begin{align*}
&= \int_{z - 1}^{1} f_{(x_2 - x_1)^2}(x)f_{(y_2 - y_1)^2}(z - x) \dx \\
&= \int_{z - 1}^{1} \left( \frac{1}{\sqrt{x}} - 1 \right) \left( \frac{1}{\sqrt{z - x}} - 1 \right) \dx \\
&= \int_{z - 1}^{1} \frac{1}{\sqrt{xz - x^2}} - \frac{1}{\sqrt{x}} - \frac{1}{\sqrt{z - x}} + 1 \dx \\
&= 2 \sin^{-1} \left( \sqrt{\frac{x}{z}} \right) + 2\sqrt{z - x} - 2\sqrt{x} + x \Big|_{z - 1}^{1} \\
&= \left( 2 \sin^{-1} \left( \sqrt{\frac{1}{z}} \right) + 2\sqrt{z - 1} - 2\sqrt{1} + 1 \right) - \left( 2 \sin^{-1} \left( \sqrt{\frac{(z - 1)}{z}} \right) + 2\sqrt{z - (z - 1)} - 2\sqrt{(z - 1)} + (z - 1) \right) \\
&= 2 \sin^{-1} \left( \sqrt{\frac{1}{z}} \right) - 2 \sin^{-1} \left( \sqrt{1 - \frac{1}{z}} \right) - z + 4\sqrt{z - 1} - 2 \\
&= 2 \sin^{-1} \left( \sqrt{\frac{1}{z}} \right) - 2 \left( \frac{\pi}{2} - \sin^{-1} \left( \sqrt{\frac{1}{z}} \right) \right) - z + 4\sqrt{z - 1} - 2 \\
&= 2 \sin^{-1} \left( \sqrt{\frac{1}{z}} \right) - \pi + 2 \sin^{-1} \left( \sqrt{\frac{1}{z}} \right) - z + 4\sqrt{z - 1} - 2 \\
&= 4 \sin^{-1} \left( \sqrt{\frac{1}{z}} \right) - z + 4\sqrt{z - 1} - 2 - \pi \\
\end{align*}

The integral of this last equation from $1$ to $t$:

\begin{align*}
&  \int_{1}^{t} 4 \sin^{-1} \left( \sqrt{\frac{1}{z}} \right) - z + 4\sqrt{z - 1} - 2 - \pi \dz \\
&= 4z \sin^{-1} \left( \sqrt{\frac{1}{z}} \right) + 4\sqrt{z-1} - \frac{1}{2} z^2 + \frac{8}{3}(z - 1)^\frac{3}{2} - (2 + \pi)z \Big|_{1}^{t} \\
&= \left( 4t \sin^{-1} \left( \sqrt{\frac{1}{t}} \right) + 4\sqrt{t-1} - \frac{1}{2} t^2 + \frac{8}{3}(t - 1)^\frac{3}{2} - (2 + \pi)t \right) \\
&  - \left( 4(1) \sin^{-1} \left( \sqrt{\frac{1}{1}} \right) + 4\sqrt{1-1} - \frac{1}{2} 1^2 + \frac{8}{3}(1 - 1)^\frac{3}{2} - (2 + \pi)(1) \right) \\
&= 4t \sin^{-1} \left( \sqrt{\frac{1}{t}} \right) + 4\sqrt{t-1} - \frac{1}{2} t^2 + \frac{8}{3}(t - 1)^\frac{3}{2} - (2 + \pi) t - \pi + \frac{5}{2} \\
\end{align*}

Putting it together:

\begin{align*}
f_{(x_2 - x_1)^2 + (y_2 - y_1)^2}(z) &=
\begin{cases}
    \pi - 4\sqrt{z} + z                                                         & 0 \leq z \leq 1 \\
    4 \sin^{-1} \left( \sqrt{\frac{1}{z}} \right) - z + 4\sqrt{z - 1} - 2 - \pi & 1 \leq z \leq 2 \\
\end{cases}
\\
F_{(x_2 - x_1)^2 + (y_2 - y_1)^2}(t) &=
\begin{cases}
    \pi t - \frac{8}{3} t^{\frac{3}{2}} + \frac{1}{2}t^2
        & 0 \leq t \leq 1 \\
    \frac{1}{3} + 4t \sin^{-1} \left( \sqrt{\frac{1}{t}} \right) + 4\sqrt{t-1} - \frac{1}{2} t^2 + \frac{8}{3}(t - 1)^\frac{3}{2} - (2 + \pi) t
        & 1 \leq t \leq 2 \\
\end{cases}
\end{align*}

\section{Probability of $d$}

\begin{align*}
F_d(t)
&= P[d \leq t] \\
&= P[\sqrt{(x_2 - x_1)^2 + (y_2 - y_1)^2} \leq t] \\
&= P[(x_2 - x_1)^2 + (y_2 - y_1)^2 \leq t^2] \\
&= F_{(x_2 - x_1)^2 + (y_2 - y_1)^2}(t^2) \\
\end{align*}

When $t \in [0, 1]$:

\begin{align*}
&= \pi (t^2) - \frac{8}{3} (t^2)^{\frac{3}{2}} + \frac{1}{2}(t^2)^2 \\
&= \pi t^2 - \frac{8}{3} t^3+ \frac{1}{2}t^4 \\
\end{align*}

When $t \in [1, \sqrt{2}]$:

\begin{align*}
&= \frac{1}{3} + 4t^2 \sin^{-1} \left( \sqrt{\frac{1}{t^2}} \right) + 4\sqrt{t^2-1} - \frac{1}{2} (t^2)^2 + \frac{8}{3}(t^2 - 1)^\frac{3}{2} - (2 + \pi) t^2 \\
&= \frac{1}{3} + 4t^2 \sin^{-1} \left( \frac{1}{t} \right) + 4\sqrt{t^2-1} - \frac{1}{2} t^4 + \frac{8}{3}(t^2 - 1)^\frac{3}{2} - (2 + \pi) t^2 \\
\end{align*}

Putting it together:

\begin{align*}
F_d(t) &=
\begin{cases}
    \pi t^2 - \frac{8}{3} t^3 + \frac{1}{2}t^4
        & 0 \leq t \leq 1 \\
    \frac{1}{3} + 4t^2 \sin^{-1} \left( \frac{1}{t} \right) + 4\sqrt{t^2-1} - \frac{1}{2} t^4 + \frac{8}{3}(t^2 - 1)^\frac{3}{2} - (2 + \pi) t^2
        & 1 \leq t \leq \sqrt{2} \\
\end{cases}
\\
f_d(z) &=
\begin{cases}
    2\pi z - 8z^2 + 2z^3
        & 0 \leq z \leq 1 \\
    8z \sin^{-1} \left( \frac{1}{z} \right) - 2z^3 + 8z\sqrt{z^2 - 1} - (4 + 2\pi) z
        & 1 \leq z \leq \sqrt{2} \\
\end{cases}
\end{align*}

\section{Probability of $r$}

\begin{align*}
F_r(t)
&= P[r \leq t] \\
&= P \left[ \frac{d}{2} \leq t \right] \\
&= P[d \leq 2t] \\
&= F_d(2t) \\
\end{align*}

When $t \in \left[ 0, \frac{1}{2} \right]$:

\begin{align*}
&= \pi (2t)^2 - \frac{8}{3} (2t)^3 + \frac{1}{2}(2t)^4 \\
&= 4\pi t^2 - \frac{64}{3}t^3 + 8t^4 \\
\end{align*}

When $t \in \left[ \frac{1}{2}, \frac{\sqrt{2}}{2} \right]$:

\begin{align*}
&= \frac{1}{3} + 4(2t)^2 \sin^{-1} \left( \frac{1}{2t} \right) + 4\sqrt{(2t)^2-1} - \frac{1}{2} (2t)^4 + \frac{8}{3}((2t)^2 - 1)^\frac{3}{2} - (2 + \pi) (2t)^2 \\
&= \frac{1}{3} + 16t^2 \sin^{-1} \left( \frac{1}{2t} \right) + 4\sqrt{4t^2-1} - 8t^4 + \frac{8}{3}(4t^2 - 1)^\frac{3}{2} - (8 + 4\pi)t^2 \\
\end{align*}

Putting it together:

\begin{align*}
F_r(t) &=
\begin{cases}
    4\pi t^2 - \frac{64}{3}t^3 + 8t^4
        & 0 \leq t \leq \frac{1}{2} \\
    \frac{1}{3} + 16t^2 \sin^{-1} \left( \frac{1}{2t} \right) + 4\sqrt{4t^2-1} - 8t^4 + \frac{8}{3}(4t^2 - 1)^\frac{3}{2} - (8 + 4\pi)t^2
        & \frac{1}{2} \leq t \leq \frac{\sqrt{2}}{2} \\
\end{cases}
\\
f_r(z) &=
\begin{cases}
    8\pi z - 64z^2 + 32z^3
        & 0 \leq z \leq \frac{1}{2} \\
    32z \sin^{-1} \left( \frac{1}{2z} \right) - 32z^3 + 32z\sqrt{4z^2 - 1} - (16 + 8\pi)z
        & \frac{1}{2} \leq z \leq \frac{\sqrt{2}}{2} \\
\end{cases}
\end{align*}

\end{document}
